all commute lemmas fixed + progress in indep_evs_commute

txn-data-consistency/EP+_Trace.thy
@@ -16,9 +16,9 @@ definition svr_ord :: "'v ev rel" where
   "svr_ord \<equiv> {(ev1, ev2). ev_key ev1 \<noteq> None \<and> ev_key ev1 = ev_key ev2}"
 
 inductive_set txn_ord :: "'v ev rel" where
-  "\<lbrakk>t = Tn_cl sn cl; m = clk\<rbrakk> \<Longrightarrow> (RInvoke cl _ sn clk, RegR _ _ _ _ _ _ m) \<in> txn_ord"
-| "\<lbrakk>t = Tn_cl sn cl; m = clk\<rbrakk> \<Longrightarrow> (WInvoke cl _ sn clk, PrepW _ _ _ _ m) \<in> txn_ord"
-| "\<lbrakk>t = Tn_cl sn cl; m = clk\<rbrakk> \<Longrightarrow> (WCommit cl _ _ sn _ clk _, CommitW _ _ _ _ _ _ m) \<in> txn_ord"
+  "\<lbrakk>t = Tn_cl sn cl; m = clk\<rbrakk> \<Longrightarrow> (RInvoke cl _ sn clk, RegR _ t _ _ _ _ m) \<in> txn_ord"
+| "\<lbrakk>t = Tn_cl sn cl; m = clk\<rbrakk> \<Longrightarrow> (WInvoke cl _ sn clk, PrepW _ t _ _ m) \<in> txn_ord"
+| "\<lbrakk>t = Tn_cl sn cl; m = clk\<rbrakk> \<Longrightarrow> (WCommit cl _ _ sn _ clk _, CommitW _ t _ _ _ _ m) \<in> txn_ord"
 | "\<lbrakk>t = Tn_cl sn cl; m = (clk, lst)\<rbrakk> \<Longrightarrow> (RegR k t _ _ clk lst _, Read cl k _ _ sn _ m) \<in> txn_ord"
 | "\<lbrakk>t = Tn_cl sn cl; mmap k = Some clk\<rbrakk> \<Longrightarrow> (PrepW k t _ clk _, WCommit cl _ _ sn _ _ mmap) \<in> txn_ord"
 | "\<lbrakk>t = Tn_cl sn cl; mmap k = Some (clk, lst)\<rbrakk> \<Longrightarrow>(CommitW k t _ _ clk lst _, WDone cl _ sn _ mmap) \<in> txn_ord"
